src/cbor/pulse/raw/everparse/CBOR.Pulse.Raw.EverParse.Det.Impl.Aux.fsti
@@ -53,7 +53,9 @@ val mk_det_raw_cbor_array_eq (y: Spec.cbor) (l: list Spec.cbor)
       Spec.unpack y == Spec.CArray l)
     (ensures
        SpecRawBase.Array? (SpecRaw.mk_det_raw_cbor y) /\
-       (SpecRawBase.Array?.v (SpecRaw.mk_det_raw_cbor y) <: list SpecRawBase.raw_data_item) == det_raw_list l)
+       (SpecRawBase.Array?.v (SpecRaw.mk_det_raw_cbor y) <: list SpecRawBase.raw_data_item) == det_raw_list l /\
+       SpecRawBase.Array?.len (SpecRaw.mk_det_raw_cbor y) ==
+         Optimal.mk_raw_uint64 (FStar.UInt64.uint_to_t (List.Tot.length l)))
 
 (* ====================================================================
    Map-entry analogues of det_raw_list. Used as the underlying
