src/cbor/pulse/raw/everparse/CBOR.Pulse.Raw.EverParse.Det.Impl.fsti
@@ -164,6 +164,8 @@ val cbor_det_map_iterator_gather (_: unit) : gather_t cbor_det_map_iterator_matc
 val cbor_det_map_iterator_next (_: unit) : map_iterator_next_t cbor_det_map_entry_match cbor_det_map_iterator_match
 val cbor_det_map_iterator_start (_: unit) : map_iterator_start_t cbor_det_match cbor_det_map_iterator_match
 
+val cbor_det_mk_array (_: unit) : mk_array_t cbor_det_match
+
 
 (* ====================================================================
    Status of original task spec items, as of latest commits in this branch
